\documentclass[a4paper, 12pt]{article}
\usepackage{amssymb, amsmath, amsthm}

\title{hw-3}
\author{Nikita Talalai}
\date{May 2023}

\newtheorem*{ex}{Exercise}
\newtheorem*{sol}{Solution}
 
\begin{document}

    \maketitle
    \centering{\section*{First Task}}

    \begin{ex}
        \begin{equation}\label{1}
            ((\lambda a.(\lambda b.b\ b)\ (\lambda b.b\ b))\ b)\  ((\lambda c.c\ b)\ (\lambda a.a))
        \end{equation}
    \end{ex}

    \begin{sol}
        \begin{equation*}
            \begin{split}
                ((\lambda a.(\lambda b.b\ b)\ (\lambda b.b\ b))\ b)\  ((\lambda c.c\ b)\ (\lambda a.a)) 
                & \xrightarrow[\beta]{} ((\lambda b.b\ b)\ (\lambda b.b\ b))\  ((\lambda c.c\ b)\ (\lambda a.a))\\
                & = \Omega\ ((\lambda c.c\ b)\ (\lambda a.a))
            \end{split}
        \end{equation*}
        \centering{Eqation \eqref{1} hasn't normal form}
    \end{sol}
    
\end{document}