\documentclass[a4paper, 12pt]{article}
\usepackage{amssymb, amsmath, amsthm}

\title{hw-3}
\author{Nikita Talalai}
\date{May 2023}

\newtheorem*{thm}{Theorem}

\begin{document}
    \maketitle

    \centering{\section*{Second Task}}

        \begin{thm}
            S K K = I
        \end{thm}
        
        \begin{proof}
            \begin{equation*}\label{xx}
                \begin{split}
                    S\ K\ K& = \overbrace{(\lambda f\ g\ x.f\ x\ (g\ x))}^{S}\
                    \overbrace{(\lambda x\ y.x)}^{K}\ \overbrace{(\lambda x\ y.x)}^{K}\\
                    & \to_\beta [f := \lambda x\ y.x]\\
                    & \to_\beta (\lambda g\ x.(\lambda x\ y.x)\ x\ (g\ x))\  (\lambda x\ y.x)\\
                    & \to_\alpha (\lambda g\ x.(\lambda x'\ y.x')\ x\ (g\ x))\  (\lambda x\ y.x)\\
                    & \to_\beta [g := \lambda x\ y.x]\\ 
                    & \to_\beta \lambda x.(\lambda x'\ y.x')\ x\ ((\lambda x\ y.x)\ x)\\
                    & \to_\alpha \lambda x.(\lambda x'\ y.x')\ x\ ((\lambda x''\ y.x'')\ x)\\
                    & \to_\beta [x' := x]\\
                    & \to_\beta \lambda x.(\lambda y.x)\ ((\lambda x''\ y.x'')\ x)\\
                    & \to_\beta [y := (\lambda x''\ y.x'')\ x]\\
                    & \to_\beta \lambda x.x\\
                    & = I
                \end{split}
            \end{equation*}
        \end{proof}
    
\end{document}